Encoding without proofs; requires the new Retract library

TM/Code/Code.v
@@ -12,12 +12,10 @@ Section Codable.
   Variable (sig: finType).
   Variable (X: Type).
 
-  Definition encoding_function := X -> list sig.
-
   Class codable :=
     mk_codable
       {
-        encode : encoding_function;
+        encode :> X -> list sig
       }.
 
   Hypothesis codable_X : codable.
@@ -25,242 +23,128 @@ Section Codable.
 End Codable.
 Arguments encode { sig } { X } { _ }.
 
+Coercion encode : codable >-> Funclass.
 
-Section Encode_Finite.
+
+Section Encode_finite.
   (* HACK: [encode true] would not work if we just define [Variable X:finType] *)
   Context `{fX: finTypeC X}.
 
-  Global Instance Encode_Finite : codable (FinType X) (FinType X) :=
+  Global Instance Encode_finite : codable (FinType X) (FinType X) :=
     {
       encode := fun x => [x];
     }.
 
-End Encode_Finite.
+End Encode_finite.
 
 (*
-Global Instance Encode_Bool : codable (FinType (EqType bool)) bool := Encode_Finite (FinType (EqType bool)).
-*)
-
+Check @Encode_finite.
 Compute encode true.
 Compute encode (Fin10: Fin.t 11).
+(* This works thanks to the coercion above *)
+Check Encode_finite true.
+Check (_ : codable _ _) _.
+*)
 
 
-Section Encode_Map.
+(** We restrict mapping of encodings to injective/retractable mappings. *)
+Section Encode_map.
   Variable (X : Type).
   Variable (sig tau : finType).
   Hypothesis (code_sig : codable sig X).
-  Variable (f : sig -> tau).
 
-  Global Instance Encode_Map : codable tau X :=
+  Variable inj : Retract sig tau.
+
+  Global Instance Encode_map : codable tau X | 100 :=
     {
-      encode x := map f (encode x);
+      encode x := map Retr_f (encode x);
     }.
   
-End Encode_Map.
+End Encode_map.
 
 
-Section Encode_Sum.
+Section Encode_sum.
   Variable (X Y : Type).
   Variable (sig tau : finType).
   Hypothesis (cX : codable sig X) (cY : codable tau Y).
 
-  Global Instance Encode_Sum : codable (FinType(EqType(bool+(sig+tau)))) (X+Y) :=
-    {
+  Check fun x => encode (x:X) : list (bool+(sig+tau)).
+  Check TRetract_inr.
+  Check _ : Retract sig (bool + (sig + tau)).
+
+  Global Instance Encode_sum : codable (FinType(EqType(bool+(sig+tau)))) (X+Y) :=
+    {|
       encode s := match s with
-                  | inl x => inl true :: Encode_Map
+                  | inl x => inl true  :: encode x
+                  | inr y => inl false :: encode y
+                  end
+    |}.
+  
+End Encode_sum.
+
+Eval cbn in encode (inl true).
+
+
+(** If [X] and [Y] are both encodable over [sig], we could also encode [X*Y] over [unit+sig]. *)
+Section Encode_pair.
+  Context (sig: finType) `{cX : codable sig X} `{cY : codable sig Y}.
+
+  Global Instance Encode_pair : codable (FinType (EqType (unit+sig))) (X*Y) :=
+    {|
+      encode '(x,y) := encode x ++ inl tt :: encode y;
+    |}.
+
+End Encode_pair.
+
+
+Section Encode_option.
+  Context (sig: finType) `{cX : codable sig X}.
+
+  Global Instance Encode_option : codable (FinType(EqType(bool+sig))) (option X) :=
+    {|
+      encode o := match o with
+                  | None => [inl false]
+                  | Some x => inl true :: encode x
+                  end;
+    |}.
+
+End Encode_option.
 
   
 
-
-  Global Instance retract_r_l : TRetract sig (bool + (sig + tau)) := Build_TRetract (tretract_compose _ _).
-  Global Instance retract_r_r : TRetract tau (bool + (sig + tau)) := Build_TRetract (tretract_compose _ _).
-
-  Definition encode_sum (a : X + Y) : list (bool + (sig + tau)) :=
-    match a with
-    | inl x => inl true  :: encode x
-    | inr y => inl false :: encode y
-    end.
-
-  Lemma encode_sum_injective :
-    forall (v1 v2 : X + Y) (r1 r2 : list (bool + (sig + tau))),
-      encode_sum v1 ++ r1 = encode_sum v2 ++ r2 -> v1 = v2 /\ r1 = r2.
-  Proof.
-    intros [x1|y1] [x2|y2] r1 r2; cbn; intros H; inv H.
-    - eapply encode_map_injective in H1 as (->&->). tauto.
-      apply retract_r_l.
-    - eapply encode_map_injective in H1 as (->&->). tauto. apply retract_r_r.
-  Qed.
-
-  Global Instance Encode_Sum : codable (FinType (EqType (bool + (sig + tau)))) (X + Y) := mk_codable encode_sum_injective.
-End Encode_Sum.
-
-
-Section Encode_Pair.
-  Variable (X Y : Type) (sig : finType).
-  Hypothesis (code_X : codable sig X) (code_Y : codable sig Y).
-
-  Definition encode_pair (v : X * Y) : list sig.
-  Proof. destruct v as (a,b). apply (encode (codable := code_X) a ++ encode (codable := code_Y) b). Defined.
-
-  Lemma encode_pair_injective :
-    forall (v1 v2 : X * Y) (r1 r2 : list sig), encode_pair v1 ++ r1 = encode_pair v2 ++ r2 -> v1 = v2 /\ r1 = r2.
-  Proof.
-    intros (a1, b1) (a2, b2) r1 r2 H. unfold encode_pair in *. rewrite <- !app_assoc in H.
-    apply encode_injective in H as (->&H). apply encode_injective in H as (->&->). auto.
-  Qed.
-
-  Global Instance Encode_Pair : codable sig (X * Y) := mk_codable encode_pair_injective.
-End Encode_Pair.
-
-Section Encode_Pair'.
-  Variable (X Y : Type) (sig tau : finType).
-
-  Hypothesis (code_X : codable sig X) (code_Y : codable tau Y).
-
-  Global Instance Encode_Pair' : codable (FinType (EqType (sig + tau)%type)) (X * Y).
-  Proof.
-    apply Encode_Pair; apply (Encode_Map _ _).
-  Defined.
-      
-End Encode_Pair'.
-
-
-Section Encode_Unit.
-  Definition encode_unit : encoding_function (FinType (EqType Empty_set)) unit := fun _ : unit => [].
-
-  Lemma encode_unit_injective :
-    forall (v1 v2 : unit) (r1 r2 : list (FinType (EqType Empty_set))), encode_unit v1 ++ r1 = encode_unit v2 ++ r2 -> v1 = v2 /\ r1 = r2.
-  Proof. intros () () r1 r2. auto. Qed.
-
-  Global Instance Encode_Unit : codable (FinType (EqType Empty_set)) unit := mk_codable encode_unit_injective.
-
-End Encode_Unit.
-
-Section Encode_Empt.
-  Definition encode_empty : encoding_function (FinType (EqType Empty_set)) Empty_set := fun devil => match devil with end.
-
-  Lemma encode_empty_injective :
-    forall (v1 v2 : Empty_set) (r1 r2 : list (FinType (EqType Empty_set))), encode_empty v1 ++ r1 = encode_empty v2 ++ r2 -> v1 = v2 /\ r1 = r2.
-  Proof. intros v1. destruct v1. Qed.
-    
-  Global Instance I_empty : codable (FinType (EqType Empty_set)) Empty_set := mk_codable encode_empty_injective.
-End Encode_Empt.
-
-Section Encode_Cast.
-  Variable sig : finType.
-  Variable (X Y : Type) (f : Y -> X).
-  Hypothesis (codeX : codable sig X).
-  Hypothesis (inj : injective f).
-
-  Lemma Encode_Cast : codable sig Y.
-  Proof.
-    esplit with (encode := fun y => encode (f y)).
-    - intros v1 v2 r1 r2 H. apply encode_injective in H as (H&->). split; eauto.
-  Defined.
-
-End Encode_Cast.
-
-Lemma Encode_Option' (X : Type) (sig : finType) : codable sig X -> codable (FinType (EqType (bool + (sig + Empty_set)))) (option X).
-Proof.
-  intros H. eapply Encode_Cast. eapply Encode_Sum.
-  - apply H.
-  - unfold finType_CS. apply Encode_Unit.
-  - now auto_inj.
-    (* eapply retract_injective. eapply tight_retract_strong.
-    eapply inversion_retract. eapply inverse_option_unit. *)
-Defined.
-
-(* Eleminate the Empty_set from above *)
-Global Instance Encode_Option (X : Type) (sig : finType) : codable sig X -> codable (FinType (EqType (bool + sig))) (option X).
-Proof.
-  intros H. eapply Encode_Map. eapply Encode_Option'; auto. eapply inversion_retract. 
-  (* (* Just for cosmetics *) Unshelve. all: unfold finType_CS. 2-3: cbn; shelve. Show Existentials. *)
-  eapply inverse_sum.
-  - auto_inj. (* eapply inverse_sum_Empty_set. *)
-  - auto_inj. (* apply inverse_id. *)
-Defined.
-
-
-Section Encode_List.
+Section Encode_list.
   Variable sig: finType.
   Variable (X : Type) (code_X : codable sig X).
 
   Fixpoint encode_list (xs : list X) : list (bool + sig) :=
     match xs with
     | nil => [inl false]
-    | x :: xs' => inl true :: encode (codable := Encode_Map code_X (@retract_inr _ _)) x ++ encode_list xs'
+    | x :: xs' => inl true :: encode x ++ encode_list xs'
     end.
 
-  Lemma encode_injective_list :
-    forall (v1 v2 : list X) (r1 r2 : list (bool + sig)), encode_list v1 ++ r1 = encode_list v2 ++ r2 -> v1 = v2 /\ r1 = r2.
-  Proof.
-    intros xs. induction xs as [ | x xs IH]; intros y2 r1 r2 H; cbn in *.
-    + destruct y2; cbn in *; try congruence; cbn in *; try now inv H.
-    + destruct y2 as [ | y ys]; cbn in *; auto.
-      * congruence.
-      * inv H. rewrite <- !app_assoc in H1.
-        eapply encode_map_injective in H1 as (->&H1). now specialize (IH _ _ _ H1) as (->&->). apply retract_inr.
-  Qed.
-
-  Global Instance Encode_List : codable (FinType (EqType (bool + sig))) (list X) := mk_codable encode_injective_list.
-
-End Encode_List.
-
-
-
-
-
-Section Encode_Nat.
-  Instance cast_nat : injective (fun n => @List.repeat unit tt n).
-  Proof.
-    hnf. intros m n. revert m. induction n; intros m H.
-    - destruct m; cbn in *; congruence.
-    - cbn in *. destruct m; cbn in *. congruence. f_equal. apply IHn. congruence.
-  Qed.
-
-  Global Instance Encode_Nat : codable (FinType (EqType bool)) nat.
-  Proof.
-    eapply Encode_Map.
-    - eapply Encode_Cast.
-      + apply Encode_List. apply Encode_Unit.
-      + apply cast_nat; auto_inj.
-    - auto_inj.
-  Defined.
-End Encode_Nat.
-
-
-Section Encode_Fin'.
-  Variable (n : nat).
-
-  Definition fin_to_nat : (Fin.t n) -> nat :=
-    fun i :  (Fin.t n) => proj1_sig (Fin.to_nat i).
+  Global Instance Encode_list : codable (FinType(EqType(bool+sig))) (list X) :=
+    {|
+      encode := encode_list;
+    |}.
   
-  Lemma fin_to_nat_injective:
-    forall x1 x2 : (Fin.t n),
-      fin_to_nat x1 = fin_to_nat x2 -> x1 = x2.
-  Proof.
-    intros x1 x2. unfold fin_to_nat. intros H.
-    f_equal. now apply Fin.to_nat_inj.
-  Qed.
-  
-  Local Instance cast_Fin : injective fin_to_nat.
-  Proof.
-    hnf. intros x1 x2. apply fin_to_nat_injective.
-  Qed.
+End Encode_list.
 
-  Local Instance Encode_Fin' : codable (FinType (EqType bool)) (Fin.t n).
-  Proof.
-    eapply Encode_Cast; [ | eapply cast_Fin ]. apply Encode_Nat.
-  Defined.
-  
-End Encode_Fin'.
 
+Section Encode_nat.
+
+  Global Instance Encode_nat : codable (FinType(EqType bool)) nat :=
+    {|
+      encode n := repeat true n ++ [false];
+    |}.
+
+End Encode_nat.
+
+
+    
 (** Test Playground *)
 
-(*
 Compute encode (Some true).
-Compute encode None.
-
+Eval cbv in encode None.
 
 Compute encode false.
 Compute encode true.
@@ -269,31 +153,15 @@ Compute encode 42.
 
 Compute encode (tt, tt).
 
-Compute ([tt;tt;tt], true).
-
-Print FinType.
-Search finTypeC Fin.t.
-Search Fin.t FinType.
-
-Require Import TM.TM.
-Check (FinType (EqType move)).
-
-Check encode (X := list (FinType (EqType move))).
-Compute encode (X := list (FinType (EqType move))) [L; N; R].
-
-Compute encode (X := FinType (EqType (Fin.t 10))) (Fin.FS (Fin.FS (Fin.FS (Fin.F1)))).
-Compute encode (codable := Encode_Fin' 10) (Fin.FS (Fin.FS (Fin.FS (Fin.F1)))).
-
-Check Encode_Pair' (Encode_List (Encode_Unit)) Encode_Unit.
-
-Compute encode ([tt;tt;tt], tt).
-
-Compute encode ([tt;tt;tt], tt, 42).
-
+Compute encode [tt;tt;tt].
 
 Compute encode (inl 42).
 Compute encode (inr 42).
-Compute encode (1, 2).
+
+Compute Encode_pair (1, 2).
+
 Compute encode [4;5].
 Compute encode (Some 4) ++ encode (Some 5) ++ encode None.
-*)
+
+Compute Encode_pair ([tt;tt;tt], true).
+Compute encode ([tt;tt;tt], tt).
